src/xor/xor.lean
@@ -45,7 +45,7 @@ def eval (α : assignment) (g : xor_gate) : bool :=
 @[simp] lemma eval_nil (α : assignment) : eval α [] = ff := rfl
 
 lemma eval_cons (α : assignment) (l : literal) (g : xor_gate) : eval α (l :: g) = bxor (literal.eval α l) (eval α g) :=
-  by simp [eval, foldr_cons, bool.bxor_comm]
+by simp [eval, foldr_cons, bool.bxor_comm]
 
 theorem eval_cons_conjunctive (α : assignment) (l : literal) (g : xor_gate) : 
   eval α (l :: g) = (literal.eval α l || eval α g) && (!(literal.eval α l) || !(eval α g)) :=
@@ -72,207 +72,269 @@ end
 theorem xor_odd_eval_tt (α : assignment) (g : xor_gate) : g.eval α = nat.bodd (g.countp (λ l, l.eval α = tt)) :=
 begin
   induction g with l ls ih,
-  split; { simp [eval] },
-  by_cases (l.eval α = tt),
-  { simp [h, ih, eval_cons] },
-  { simp at h, simp [h, ih, eval_cons] }
+  { simp },
+  { rcases bool_by_cases (l.eval α) with h | h;
+    { simp [eval_cons, h, ih] } }
 end
 
+-- This is a shortcut of the above that uses gate.to_clause instead
+-- NOTE that the to_clause is essentially an identity operation, but if sets/permuations are
+-- used instead, the proof may grow more complex
 theorem xor_odd_eval_tt2 (α : assignment) (g : xor_gate) : g.eval α = nat.bodd (g.to_clause.count_tt α) :=
 begin
   induction g with l ls ih,
   { simp [to_clause] },
-  {
-    by_cases (l.eval α = tt),
+  { rcases bool_by_cases (l.eval α);
     { rw ← gate_eq_clause ls at ih,
-      simp [to_clause, eval_cons, count_tt_cons, bool.to_nat, h, ih] },
-    { simp at h,
-      rw ← gate_eq_clause ls at ih,
       simp [to_clause, eval_cons, count_tt_cons, bool.to_nat, h, ih] } }
 end
 
+/-! ## Naive encoding, simple version -/
+
 -- Let's start easier: turning a list of natural numbers into a cnf form
--- We use explode.explode, which takes in a list of nats. Alternatively, we take a list of ints and get tricky with negatives meaning flipped
--- Note the return value of explode is list clause, which is cnf
+-- The naive encoding returns a formula with all possible clauses with an even number of negated literals
+-- Because we are using natural numbers, i.e. positive literals, we want an even number of negative literals
 def nat_to_xor_cnf : list nat → cnf
 | []        := [[]]
 | (n :: ns) := (explode ns).map (λ c, cond (nat.bodd c.count_neg = ff) ((Pos n) :: c) ((Neg n) :: c))
 
--- Riskier, but what else can you do?
 theorem mem_explode_of_mem_nat_to_xor :
   ∀ {ns : list nat}, ∀ {c : clause}, c ∈ nat_to_xor_cnf ns → c ∈ explode ns
 | []        := by simp [nat_to_xor_cnf]
 | (n :: ns) := begin
   simp [nat_to_xor_cnf, mem_map, mem_append],
   intros c hc,
-  by_cases c.count_neg.bodd = tt,
-  { simp [h], have : (Pos n).var = n, simp [var],
-    exact mem_explode_cons_of_lit c hc this },
-  { simp [bool_eq_false h], have : (Neg n).var = n, simp [var],
-    exact mem_explode_cons_of_lit c hc this }
+  have : (Pos n).var = n ∧ (Neg n).var = n, simp [var], -- Make into literal lemma?
+  rcases bool_by_cases (c.count_neg.bodd) with h | h;
+  { simp [h, mem_explode_cons_of_lit c hc, this] }
 end
 
-theorem nat_to_xor_cnf_length {ns : list nat} : ns ≠ [] → length (nat_to_xor_cnf ns) = 2^(length ns - 1) :=
-begin
-  cases classical.em (ns = nil); intro hns,
-  { exact absurd h hns },
-  { rcases exists_cons_of_ne_nil hns with ⟨w, ⟨l, rfl⟩⟩, 
-    simp only [nat_to_xor_cnf, length_map, length_cons, length_explode, nat.succ_sub_one] }
-end
+theorem length_nat_to_xor_cnf : ∀ {ns : list nat}, ns ≠ [] → length (nat_to_xor_cnf ns) = 2^(length ns - 1)
+| []        := by { contradiction }
+| (n :: ns) := by simp [nat_to_xor_cnf, length_explode]
+
+theorem length_nat_to_xor_cnf_pos : ∀ {ns : list nat}, ns ≠ [] → length (nat_to_xor_cnf ns) > 0
+| []        := by { contradiction }
+| (n :: ns) := by simp [length_nat_to_xor_cnf]
 
 theorem exists_mem_nat_to_xor_of_ne_nil {ns : list nat} : ns ≠ [] → ∃ (c : clause), c ∈ nat_to_xor_cnf ns :=
-begin
-  induction ns with m ms ih,
-  { contradiction },
-  { intro _,
-    by_cases hms : ms = [],
-    { use (Pos m) :: [],
-      simp [hms, nat_to_xor_cnf] },
-    { 
-      rcases ih hms with ⟨c, hc⟩,
-      by_cases nat.bodd c.count_neg = ff,
-      { use (Pos m :: c),
-        simp [nat_to_xor_cnf],
-        use c,
-        simp [mem_explode_of_mem_nat_to_xor hc, h] },
-      { use (Neg m :: c),
-        simp [nat_to_xor_cnf],
-        use c,
-        simp [mem_explode_of_mem_nat_to_xor hc, h] } } }
-end
+assume h, exists_mem_of_length_pos (length_nat_to_xor_cnf_pos h)
 
 theorem map_var_eq_of_mem_nat_to_xor : ∀ {ns : list nat}, ∀ {c : clause}, c ∈ nat_to_xor_cnf ns → c.map var = ns
-| []        := by { simp [nat_to_xor_cnf] }
+| []        := by simp [nat_to_xor_cnf]
 | (n :: ns) := begin
   simp [nat_to_xor_cnf],
   intros c hc,
-  by_cases c.count_neg.bodd = ff;
+  rcases bool_by_cases c.count_neg.bodd;
   { simp [h, var, map_var_eq_of_mem_explode hc] }
 end
 
--- Can be shortened to one or two lines given aboce theorem, as sim. is weaker
-theorem map_var_sim_of_mem_nat_to_xor : ∀ (ns : list nat), ∀ (c : clause), c ∈ nat_to_xor_cnf ns → c.map var ~ ns
-| []        := by { simp [nat_to_xor_cnf] }
+theorem mem_nat_to_xor_of_even_negation_of_map_var_eq : ∀ {ns : list nat}, ∀ {c : clause}, 
+  c.map var = ns → (nat.bodd c.count_neg = ff) → c ∈ nat_to_xor_cnf ns
+| []        := by simp [nat_to_xor_cnf]
 | (n :: ns) := begin
-  simp only [nat_to_xor_cnf, mem_map, mem_append],
-  rintros c ⟨a, ⟨ha1, ha2⟩⟩,
-  by_cases a.count_neg.bodd = tt,
-  { simp [h] at ha2, simp [← ha2, var, map_var_sim_of_mem_explode a ha1] },
-  { simp [bool_eq_false h] at ha2, simp [← ha2, var, map_var_sim_of_mem_explode a ha1] }
-end
-
-theorem exists_mem_explode_sim_of_mem_nat_to_xor {ns : list nat} : 
-  ∀ (c : clause), c ∈ nat_to_xor_cnf ns → ∃ cl ∈ explode ns, c ~ cl :=
-assume c h, mem_explode_sim_of_map_var_sim c (map_var_sim_of_mem_nat_to_xor ns c h)
-
-
-
--- Technically not a proof by induction, fix later?
-theorem nat_to_xor_cnf_contains_all_even_negated_clauses {ns : list nat} :
-  ∀ {c : clause}, c.map var = ns → (nat.bodd c.count_neg = ff) → c ∈ nat_to_xor_cnf ns :=
-begin
-  induction ns with m ms ih,
-  { simp [nat_to_xor_cnf] },
-  { intros c hc,
+  intros c hc,
   rcases exists_cons_of_map_cons hc with ⟨l, ls, rfl, hl, hls⟩,
   rcases pos_or_neg_of_var_eq_nat hl with rfl | rfl;
   { simp [count_neg_cons, is_neg, bool.to_nat, nat_to_xor_cnf],
     intro hcount, use ls,
-    simp [hcount, mem_explode_of_map_var_eq hls] } }
+    simp [hcount, mem_explode_of_map_var_eq hls] }
 end
 
--- Not really induction, switch later
-theorem even_negation_of_mem_nat_to_xor {ns : list nat} :
-  ∀ {c : clause}, c.map var = ns → c ∈ nat_to_xor_cnf ns → nat.bodd c.count_neg = ff :=
-begin
-  induction ns with m ms ih,
-  { simp },
+theorem even_negation_of_mem_nat_to_xor_of_map_var_eq : ∀ {ns : list nat}, ∀ {c : clause}, 
+  c.map var = ns → c ∈ nat_to_xor_cnf ns → nat.bodd c.count_neg = ff
+| []        := by simp
+| (n :: ns) := begin
   intros c hc hxor,
   simp [nat_to_xor_cnf] at hxor,
   rcases hxor with ⟨a, ha, hacons⟩,
   rcases exists_cons_of_map_cons hc with ⟨l, ls, rfl, hl, hls⟩,
-  by_cases a.count_neg.bodd = ff,
+  rcases bool_by_cases a.count_neg.bodd with h | h;
   { simp [h] at hacons,
     simp [← hacons, count_neg_cons, is_neg, bool.to_nat, h] },
-  { simp [h] at hacons,
-    simp at h,
-    simp [← hacons, count_neg_cons, is_neg, bool.to_nat, h] }
 end
 
 theorem even_negation_iff_mem_nat_to_xor {ns : list nat} {c : clause} (hc : c.map var = ns) :
   c ∈ nat_to_xor_cnf ns ↔ nat.bodd c.count_neg = ff :=
-⟨even_negation_of_mem_nat_to_xor hc, nat_to_xor_cnf_contains_all_even_negated_clauses hc⟩
+⟨even_negation_of_mem_nat_to_xor_of_map_var_eq hc,
+  mem_nat_to_xor_of_even_negation_of_map_var_eq hc⟩
 
-theorem nat_to_xor_cnf_contains_no_odd_negated_clauses {ns : list nat} :
-  ∀ {c : clause}, c.map var = ns → (nat.bodd c.count_neg = tt) → c ∉ nat_to_xor_cnf ns :=
+theorem not_mem_nat_to_xor_cnf_of_odd_negation_of_map_var_eq {ns : list nat} {c : clause} :
+  c.map var = ns → (nat.bodd c.count_neg = tt) → c ∉ nat_to_xor_cnf ns :=
 begin
-  intros c hc hcount,
-  by_cases c ∈ nat_to_xor_cnf ns, -- This is a little cheesy, but I want to show contradiction
-  { have red := even_negation_of_mem_nat_to_xor hc h,
-    rw hcount at red,
-    exact absurd red (ne.symm ff_eq_tt_eq_false) },
-  { exact h }
+  intros hc hcount,
+  by_contradiction,
+  exact absurd_bool hcount (even_negation_of_mem_nat_to_xor_of_map_var_eq hc h)
 end
 
 -- TODO move the c.map var assumption into the ns list nat portion since the above need it too
-theorem odd_negation_of_not_mem_nat_to_xor {ns : list nat} :
-  ∀ {c : clause}, c.map var = ns → c ∉ nat_to_xor_cnf ns → nat.bodd c.count_neg = tt :=
+theorem odd_negation_of_not_mem_nat_to_xor_of_map_var_eq {ns : list nat} {c : clause} (hc : c.map var = ns) :
+  c ∉ nat_to_xor_cnf ns → nat.bodd c.count_neg = tt :=
 begin
-  intros c hc,
   contrapose,
   simp,
-  intro hcount,
-  exact nat_to_xor_cnf_contains_all_even_negated_clauses hc hcount
+  exact (even_negation_iff_mem_nat_to_xor hc).mpr
 end
 
 theorem odd_negation_iff_not_mem_nat_to_xor {ns : list nat} {c : clause} (hc : c.map var = ns) :
   c ∉ nat_to_xor_cnf ns ↔ nat.bodd c.count_neg = tt :=
-⟨odd_negation_of_not_mem_nat_to_xor hc, nat_to_xor_cnf_contains_no_odd_negated_clauses hc⟩
-
--- TODO clean up, e.g. by apply
-theorem true_forward {α : assignment} : ∀ {ns : list nat} (hnodup: ns.nodup), eval α (ns.map Pos) = tt → cnf.eval α (nat_to_xor_cnf ns) = tt
-| []        := by simp
-| (n :: ns) := begin
-  intros hnsnodup h,
-  have red := xor_odd_eval_tt2 α (map Pos (n :: ns)),
-  rw h at red,
-  rw ← gate_eq_clause (map Pos (n :: ns)) at red,
-  have : ∀ (c : clause), c ∈ nat_to_xor_cnf (n :: ns) → clause.eval α c = tt,
-  { intros c hc,
-    have mapvareq : map var c = (n :: ns), from map_var_eq_of_mem_nat_to_xor hc,
-    have : nat.bodd c.count_neg = ff, from even_negation_of_mem_nat_to_xor mapvareq hc,
-    have neq : nat.bodd (count_tt α (map Pos (n :: ns))) ≠ nat.bodd c.count_neg,
-      from neq_of_ff_of_tt (eq.symm red) this,
-    exact eval_tt_of_opposite_parity (cons_ne_nil n ns) hnsnodup mapvareq neq },
-  exact eval_tt_iff_clauses_tt.mpr this
-end
-
--- TODO clean up
-theorem false_forward {α : assignment} : ∀ {ns : list nat} (hnodup : ns.nodup), eval α (ns.map Pos) = ff → cnf.eval α (nat_to_xor_cnf ns) = ff
-| []        := by simp [nat_to_xor_cnf]
-| (n :: ns) := begin
-  intros hnsnodup h,
-  have red := xor_odd_eval_tt2 α (map Pos (n :: ns)),
-  rw h at red,
-  rw ← gate_eq_clause (map Pos (n :: ns)) at red,
-  apply eval_ff_iff_exists_clause_ff.mpr,
-  have : count_tt α (map Pos (n :: ns)) = count_neg (falsify α (n :: ns)), 
-    from count_tt_pos_eq_count_neg_falsify α (n :: ns),
-  have : nat.bodd (count_tt α (map Pos (n :: ns))) = nat.bodd (count_neg (falsify α (n :: ns))), 
-    from congr_arg nat.bodd this,
-  rw ← red at this,
-  have mapvareq := nat_to_xor_cnf_contains_all_even_negated_clauses (map_var_falsify_eq_list α (n :: ns)) this.symm,
-  use (falsify α (n :: ns)),
-  simp [mapvareq, eval_ff_of_falsify α (n :: ns)]
-end
+⟨odd_negation_of_not_mem_nat_to_xor_of_map_var_eq hc, 
+  not_mem_nat_to_xor_cnf_of_odd_negation_of_map_var_eq hc⟩
 
 -- We prove that the naive encoding is equivalent to an XOR gate of all positive literals
-theorem nat_to_xor_cnf_correct (α : assignment) {ns : list nat} (hns : ns.nodup) : 
-  cnf.eval α (nat_to_xor_cnf ns) = eval α (ns.map Pos) :=
+theorem nat_to_xor_cnf_correct (α : assignment) : ∀ {ns : list nat}, 
+  ns.nodup → cnf.eval α (nat_to_xor_cnf ns) = eval α (ns.map Pos)
+| []        := by simp [nat_to_xor_cnf]
+| (n :: ns) := begin
+  intro hnodup,
+  have red := xor_odd_eval_tt2 α (map Pos (n :: ns)),
+  rcases bool_by_cases (eval α (map Pos (n :: ns))) with h | h;
+  rw [h, ← gate_eq_clause (map Pos (n :: ns))] at red; rw h,
+  -- tt case: Parities of α and clause tt evals means all clauses are true
+  { apply eval_tt_iff_clauses_tt.mpr,
+    intros c hc,
+    have mve := map_var_eq_of_mem_nat_to_xor hc,
+    have neq := neq_of_ff_of_tt (eq.symm red) ((even_negation_iff_mem_nat_to_xor mve).mp hc),
+    exact eval_tt_of_opposite_parity (cons_ne_nil n ns) hnodup mve neq },
+  -- ff case: We generate a false clause and show it is in the encoded formula
+  { apply eval_ff_iff_exists_clause_ff.mpr,
+    use (falsify α (n :: ns)),
+    split,
+    { apply (even_negation_iff_mem_nat_to_xor (map_var_falsify_eq_list α (n :: ns))).mpr,
+      have oddeq := congr_arg nat.bodd (count_tt_pos_eq_count_neg_falsify α (n :: ns)),
+      rw ← red at oddeq,
+      exact oddeq.symm },
+    { exact eval_ff_of_falsify α (n :: ns) } }
+end
+
+/-! # More complex encoding -/
+
+/-
+The above encoding assumed that the list of interest were only positive literals.
+Here, we generalize and prove the encoding valid with general lists of literals.
+The encoding is generated by counting "flips" between clauses rather than negations of literals.
+-/
+def xor_cnf : list literal → cnf
+| []        := [[]]
+| (l :: ls) := (explode (map var ls)).map (λ c, cond (nat.bodd (c.count_flips (ls)) = ff) (l :: c) (l.flip :: c))
+
+theorem mem_explode_of_mem_xor_cnf :
+  ∀ {ls : list literal} {c : clause}, c ∈ xor_cnf ls → c ∈ explode (map var ls)
+| []        := by simp [xor_cnf]
+| (l :: ls) := begin
+  simp [xor_cnf, explode],
+  intros c hc,
+  rcases exists_nat_of_lit l with ⟨n, (rfl | rfl)⟩;
+  rcases bool_by_cases (nat.bodd (c.count_flips ls)) with h | h,
+  { right, use c, simp [h, hc, var, literal.flip] },
+  { left, use c, simp [h, hc, var, literal.flip] },
+  { left, use c, simp [h, hc, var, literal.flip] },
+  { right, use c, simp [h, hc, var, literal.flip] }
+end
+
+theorem length_xor_cnf : ∀ {ls : list literal}, ls ≠ [] → length (xor_cnf ls) = 2^(length ls - 1)
+| []        := by { contradiction }
+| (l :: ls) := by simp [xor_cnf, length_explode]
+
+theorem length_xor_cnf_pos : ∀ {ls : list literal}, ls ≠ [] → length (xor_cnf ls) > 0
+| []        := by { contradiction }
+| (l :: ls) := by simp [length_xor_cnf]
+
+theorem exists_mem_xor_cnf_of_ne_nil {ls : list literal} : ls ≠ [] → ∃ (c : clause), c ∈ xor_cnf ls :=
+assume h, exists_mem_of_length_pos (length_xor_cnf_pos h)
+
+theorem map_var_eq_of_mem_xor_cnf {ls : list literal} : ∀ {c : clause}, c ∈ xor_cnf ls → map var c = map var ls :=
 begin
-  rcases bool_by_cases (eval α (map Pos ns)) with h | h,
-  { simp [h, true_forward hns] },
-  { simp [h, false_forward hns] }
+  induction ls with l ls ih,
+  { simp [xor_cnf] },
+  { simp [xor_cnf],
+    intros c hc,
+    rcases bool_by_cases (nat.bodd (c.count_flips ls)) with h | h;
+    { simp [h, map_var_eq_of_mem_explode hc, var_flip_eq_var l] } }
+end
+
+theorem mem_xor_cnf_of_even_flips_of_map_var_eq : ∀ {ls : list literal}, ∀ {c : clause},
+  map var c = map var ls → (nat.bodd (c.count_flips ls) = ff) → c ∈ xor_cnf ls
+| []        := by simp [xor_cnf]
+| (l :: ls) := begin
+  simp [xor_cnf, map_cons],
+  intros c hc hcount,
+  rcases exists_cons_of_map_cons hc with ⟨d, ds, rfl, hd, hds⟩,
+  use ds,
+  rcases bool_by_cases (nat.bodd (count_flips ds ls)) with htt | hff,
+  { by_cases l.flip = d,
+    { simp [htt, mem_explode_of_map_var_eq hds, hd, h] },
+    { simp [count_flips, ne.symm (ne_flip_of_flip_ne h)] at hcount,
+      exact absurd_bool htt hcount } },
+  { by_cases l.flip = d,
+    { simp [count_flips, eq_flip_of_flip_eq h] at hcount,
+      exact absurd_bool hcount hff },
+    { simp [hff, mem_explode_of_map_var_eq hds, hd, eq_of_flip_ne_of_var_eq hd.symm h] } }
+end
+
+theorem even_flips_of_mem_xor_cnf_of_map_var_eq : ∀ {ls : list literal}, ∀ {c : clause},
+  c.map var = map var ls → c ∈ xor_cnf ls → nat.bodd (count_flips c ls) = ff
+| []        := by simp [xor_cnf]
+| (l :: ls) := begin
+  intros c hc hxor,
+  simp [xor_cnf] at hxor,
+  rcases hxor with ⟨a, ha, hacons⟩,
+  rcases exists_cons_of_map_cons hc with ⟨c, cs, rfl, hc2, hcs⟩,
+  rcases bool_by_cases (nat.bodd (count_flips a ls)) with h | h;
+  { simp [h] at hacons,
+    simp [← hacons, count_flips, is_neg, bool.to_nat, h, eq_flip_flip _, ne_flip_self] }
+end
+
+theorem even_flips_iff_mem_xor_cnf {ls : list literal} {c : clause} (hc : c.map var = map var ls) :
+  nat.bodd (count_flips c ls) = ff ↔ c ∈ xor_cnf ls :=
+⟨mem_xor_cnf_of_even_flips_of_map_var_eq hc, even_flips_of_mem_xor_cnf_of_map_var_eq hc⟩
+
+theorem not_mem_xor_cnf_of_odd_flips_of_map_var_eq {ls : list literal} {c : clause} :
+  map var c = map var ls → (nat.bodd (count_flips c ls)) = tt → c ∉ xor_cnf ls :=
+begin
+  intros hc hcount,
+  by_contradiction,
+  exact absurd_bool hcount ((even_flips_iff_mem_xor_cnf hc).mpr h)
+end
+
+theorem odd_flips_of_not_mem_xor_cnf_of_map_var_eq {ls : list literal} {c : clause} :
+  map var c = map var ls → c ∉ xor_cnf ls → (nat.bodd (count_flips c ls)) = tt :=
+begin
+  intro hc,
+  contrapose,
+  simp,
+  exact (even_flips_iff_mem_xor_cnf hc).mp
+end
+
+theorem odd_flips_iff_not_mem_xor_cnf {ls : list literal} {c : clause} (hc : map var c = map var ls) :
+  nat.bodd (count_flips c ls) = tt ↔ c ∉ xor_cnf ls :=
+⟨not_mem_xor_cnf_of_odd_flips_of_map_var_eq hc, odd_flips_of_not_mem_xor_cnf_of_map_var_eq hc⟩
+
+-- A restatement of the above theorem in a more general way
+-- Alternatively, the assignment can be manipulated by flipping the correct literals
+theorem xor_cnf_correct (α : assignment) : ∀ {ls : list literal},
+  (map var ls).nodup → cnf.eval α (xor_cnf ls) = eval α ls
+| []        := by simp [xor_cnf]
+| (l :: ls) := begin
+  intro hnodup,
+  have red := xor_odd_eval_tt2 α (l :: ls),
+  rcases bool_by_cases (eval α (l :: ls)) with h | h;
+  rw [h, ← gate_eq_clause (l :: ls)] at red; rw h,
+  { apply eval_tt_iff_clauses_tt.mpr,
+    intros c hc,
+    have mve := map_var_eq_of_mem_xor_cnf hc,
+    have neqodd := neq_of_ff_of_tt (eq.symm red) ((even_flips_iff_mem_xor_cnf mve).mpr hc),
+    have neq := ne_of_apply_ne nat.bodd neqodd,
+    rw count_flips_comm at neq,
+    exact eval_tt_of_neq_flips (cons_ne_nil l ls) hnodup c mve.symm neq },
+  { apply eval_ff_iff_exists_clause_ff.mpr,
+    use (falsify α (map var (l :: ls))),
+    split,
+    { rw ← count_flips_falsify_eq_count_tt α (l :: ls) at red,
+      rw count_flips_comm at red,
+      apply (even_flips_iff_mem_xor_cnf (map_var_falsify_eq_list α (map var (l :: ls)))).mp,
+      exact red.symm },
+    { exact eval_ff_of_falsify α (map var (l :: ls)) } }
 end
 
 end xor_gate
